* 6.2.3
  There are two possible solutions to this problem that maintain the requirement that $-b<r<b$. \\
  The first one is found by multiplying both sides of the division algorithm by $-1$: $-a=(-q)b+(-r)$. \\
  The second one is: $-a=-(q+1)b+(b-r)$, which is found by multiplying both sides by $-1$, then adding $b-b$ to the RHS and factoring.
* 6.2.5
  $(4\cdot 4)|8$, however $8$ does not divide $4$.
* 6.2.14
  #+BEGIN_LaTeX
    \begin{proof}
      by contradiction. \\
      Assume that $r+s$ and $s$ are not coprime.
      This means that there exists $d>1\in\Z$ s.t. $d|s$ and $d|(r+s)$.
      \begin{align*}
        &\implies \exists m,n\in\Z\ s.t.\ s=dm \land r+s=dn \\
        (r+s)-s &= dn-dm &&\tag{subtract both equations} \\
        r &= d(n-m) \\
        &\implies d|r \\
        d|r \land d|s \land d>1 &\implies \text{r and s are not co-prime} \\
        &\rightarrow\leftarrow
      \end{align*}
      Which means that $d=1$ which means that $r+s$ and $s$ must be relatively prime. $\qedhere$
    \end{proof}
  #+END_LaTeX
* 6.2.18
#+BEGIN_LaTeX
  \begin{proof}
    by contradiction. \\
    Assume $(a,b)$ and $(a,c)$ are not relatively prime.
    \begin{align*}
      &\implies \exists d\in\Z\ s.t.\ d|(a,b)\land d|(a,c) \\
      &\implies d|a, d|b, d|c &&\tag{Since d divides their gcd} \\
      &d>1\land d|b\land d|c \rightarrow\leftarrow &&\tag{Since b and c are co-prime} \\
      &\implies d=1 &&\qedhere
    \end{align*}
  \end{proof}
#+END_LaTeX
